Add more comments

RoboChart/examples/RoboChart_ChemicalDetector_autonomous/RoboChart_ChemicalDetector_autonomous.thy
@@ -2,7 +2,9 @@ section \<open> Animation of the autonomous chemical detector RoboChart model \<
 text \<open> This theory aims for animation of the autonomous chemical detector RoboChart model 
 (Version 4.0)\footnote{\url{https://robostar.cs.york.ac.uk/case_studies/autonomous-chemical-detector/autonomous-chemical-detector.html#version4}}
 based on its CSP semantics. This model is obsolete and cannot be supported in the current 
-RoboTool v2.0, and so we have updated it. 
+RoboTool v2.0, and so we have updated it. The update includes a correction of an error in the 
+definition of the @{text intensity} function, a removal of the unnecessary transition from 
+@{text Avoiding} to @{text Going} in the @{text Movement} state machine, and other changes are minor.
 \<close>
 theory RoboChart_ChemicalDetector_autonomous
   imports "RoboChart_ChemicalDetector_autonomous_general"
@@ -10,7 +12,20 @@ theory RoboChart_ChemicalDetector_autonomous
     "RoboChart_ChemicalDetector_autonomous_microcontroller"
 begin
 
-subsection \<open> Module \<close>
+text \<open>We structure the theory as follows. In Sect.~\ref{ssec:chem_general}, we give the general 
+definitions. Sects.~\ref{ssec:chem_chemical} and~\ref{ssec:chem_location} define types and 
+functions in the @{text Chemical} and @{text Location} packages of the model. The @{text GasAnalysis} 
+state machine and the @{text MainController} controller are defined in 
+Sects.~\ref{ssec:chem_gasanalysis} and~\ref{ssec:chem_maincontroller}. Then we present general 
+definitions of the @{text Movement} state machine, including the state machine defined operation 
+@{text changeDirection}, in Sect.~\ref{ssec:chem_movement_general}. 
+Afterwards, the operation and @{text Movement} are defined in 
+Sects.~\ref{ssec:chem_changedirection_op} and~\ref{ssec:chem_movement}, and @{text MicroController} 
+is defined in Sect.~\ref{ssec:chem_microcontroller}. Finally, the module @{text mod0} is defined in 
+Sect.~\ref{ssec:chem_module}.
+\<close>
+
+subsection \<open> Module \label{ssec:chem_module}\<close>
 chantype Chan_ChemicalDetector =
   terminate :: unit 
   flag :: "InOut"
@@ -123,7 +138,7 @@ definition D__ChemicalDetector where
 definition "D_ChemicalDetector_sim = D__ChemicalDetector 0"
 animate1 D_ChemicalDetector_sim
 
-subsection \<open> Export code \<close>
+subsubsection \<open> Export code \<close>
 export_code
   D__ChemicalDetector
   in Haskell 
