RoboChart/examples/RoboChart_ChemicalDetector_autonomous/RoboChart_ChemicalDetector_autonomous_general.thy
@@ -4,32 +4,51 @@ theory RoboChart_ChemicalDetector_autonomous_general
           "Z_Toolkit.Bounded_List"
 begin
 
-subsection \<open> General definitions \<close>
+subsection \<open> General definitions \label{ssec:chem_general}\<close>
 text \<open>The values below for the instantiation of @{term robochart_confs} come from the 
-@{verbatim "instantiation.csp"} file \<close>
+@{verbatim "instantiation.csp"}.
+\<close>
 interpretation rc: robochart_confs "-2" "2" "2" "0" "1".
 
-subsubsection \<open> Constants \<close>
-
-subsubsection \<open> Types \<close>
-
+subsection \<open> Chemical package \label{ssec:chem_chemical}\<close>
 text \<open> @{text Chem} from the @{text Chemical} package in the model is a @{text PrimitiveType}, 
 similar to a given type in Z. 
 In CSP, it is @{verbatim "nametype Chem = {0,1}"}. A named type in CSP simply associates a type 
-name with a set of values.
+name with a set of values. Therefore, a set of two integer numbers is chosen as a type for @{text Chem} 
+in CSP. 
+If we translate primitive types from the CSP code, we need to deal with set expressions, which is 
+more complex, and also lose the information that @{text Chem} is a primitive type. For this reason,
+the translation (no matter manual or automatic) should not be directly from the generated CSP code, 
+and should start from RoboChart models.
+
+Here, we introduce a generic way to define finite primitive types (as for model checking of CSP 
+semantics). The type variable @{typ 'a} is finite, and such one example is the numeral type @{typ 2}
+ (@{text "2 Chemical_Chem"}) which contains two elements: @{term "0::2"} and @{term "1::2"}. 
+And @{value "2::2"} is just equal to @{value "0::2"}.
+
+Similar to the CSP representation of named types, the use of a numeral type for @{typ 'a} also 
+enables the elements of this type can be compared.
 \<close>
 datatype ('a::finite) Chemical_Chem = Chemical_ChemC 'a
 
+text \<open>@{term Chemical_Chem2_set} corresponds to the named type @{verbatim Chem} in CSP. It is also a 
+set contains two elements: 0 and 1, through an implementation of sets by lists 
+(@{term Chemical_Chem2_list}). 
+\<close>
 abbreviation "Chemical_Chem2_list \<equiv> [Chemical_ChemC (0::2), Chemical_ChemC (1::2)]"
 \<comment> \<open> Use abbreviation (instead of definition) here, otherwise it cannot pattern match a list based 
 set\<close>
 abbreviation "Chemical_Chem2_set \<equiv> set Chemical_Chem2_list"
 
+text \<open>For @{text Chem}, a value (@{text "0::2"}) denotes no gas detected. Otherwise, a gas is 
+detected. 
+\<close>
 definition Chemical_Chem_is_zero::"(2 Chemical_Chem) \<Rightarrow> bool" where
 "Chemical_Chem_is_zero x = (if x = (Chemical_ChemC (0::2)) then True else False)"
 
 value "Chemical_Chem_is_zero (Chemical_ChemC (3::2))"
 
+text \<open>The definition of the @{text Intensity} type is similar to that of @{text Chem}. \<close>
 datatype ('a::finite) Chemical_Intensity = Chemical_IntensityC 'a
 
 abbreviation "Chemical_Intensity2_list \<equiv> [Chemical_IntensityC (0::2), Chemical_IntensityC 1]"
@@ -38,28 +57,37 @@ abbreviation "Chemical_Intensity2_set \<equiv> set Chemical_Intensity2_list"
 definition Chemical_Intensity_is_zero::"(2 Chemical_Intensity) \<Rightarrow> bool" where
 "Chemical_Intensity_is_zero x = (if x = (Chemical_IntensityC (0::2)) then True else False)"
 
+text \<open>The use of a numeral type for a finite type in the definition of @{term Chemical_Intensity}, 
+for example @{typ 2} here, makes the values in this type is comparable. \<close>
 fun Chemical_goreq :: "2 Chemical_Intensity \<Rightarrow> 2 Chemical_Intensity \<Rightarrow> bool" where
 "Chemical_goreq (Chemical_IntensityC x) (Chemical_IntensityC y) = (x \<ge> y) "
 
-text \<open> In CSP, LSeq(T,n) from core_defs.csp can be used as a type or an expression. In this 
-RoboChart model, it is used as a type, parametrised by n. We use bounded_list to implement it, 
-such as @{typ "int blist[2]"} for LSeq(int, 2).
-\<close>
+text \<open> In CSP, @{verbatim "LSeq(T,n)"} from @{verbatim "core_defs.csp"} can be used as a type or 
+an expression. In this RoboChart model, it is used as a type, parametrised by $n$. We use 
+@{term Bounded_List} to implement it, such as @{typ "int blist[2]"} for @{verbatim "LSeq(int, 2)"}. 
 
+The @{term "lseq s n"} function below gives a list of the all bounded lists of which each contains 
+elements from the list @{term s} only and has its length equal to @{term n}. 
+\<close>
 fun lseq where
 "lseq s 0 = [[]]" |
 "lseq s (Suc 0) = [[q]. q \<leftarrow> s]" |
 "lseq s (Suc n) = [q # qs. q \<leftarrow> s, qs \<leftarrow> (lseq s n)]"
 
+text \<open>The @{term "lseqn s n"} function gives a list of the all bounded lists of which each contains 
+elements from the list @{term s} only and has its length less than or equal to @{term n}. 
+\<close>
 fun lseqn where
 "lseqn s 0 = lseq s 0" |
 "lseqn s (Suc n) = lseqn s n @ (lseq s (Suc n))"
 
-text \<open> Make a bounded list from the supplied list, a set of all possible elements. \<close>
+text \<open> The @{term "mk_blist n s"} defines a list of the all bounded lists from the supplied list 
+@{text s}, a set of all possible elements, and the length of each bounded list is less than or equal 
+to @{text n}.\<close>
 definition mk_blist :: "'n itself \<Rightarrow> 'a list \<Rightarrow> ('a blist['n::finite]) list" where
 "mk_blist _ xs = map (bmake TYPE('n)) (lseqn xs CARD('n))"
 
-subsection \<open> Chemical package \<close>
+
 datatype Chemical_Status = 
   Chemical_Status_noGas | Chemical_Status_gasD
 
@@ -74,7 +102,6 @@ abbreviation "Chemical_Angle_list \<equiv> [Chemical_Angle_Left, Chemical_Angle_
   Chemical_Angle_Back, Chemical_Angle_Front]"
 abbreviation "Chemical_Angle_set \<equiv> set Chemical_Angle_list"
 
-text \<open> The angle function \<close>
 definition Chemical_angle :: "nat \<Rightarrow> Chemical_Angle" where
 "Chemical_angle x = (if x > 0 then Chemical_Angle_Right else Chemical_Angle_Front)"
 
@@ -88,17 +115,13 @@ definition Chemical_GasSensor2_list :: "Chemical_GasSensor2 list" where
 "Chemical_GasSensor2_list \<equiv> 
   [\<lparr>c = cc, i = ii\<rparr>. cc \<leftarrow> Chemical_Chem2_list, ii \<leftarrow> Chemical_Intensity2_list]"
 
+text \<open>The @{term lseq_gassensor_enum} defines a list of the all bounded lists of which each contains 
+up to 2 records of type @{term Chemical_GasSensor2}.\<close>
 abbreviation "lseq_gassensor_enum \<equiv> mk_blist TYPE(2) Chemical_GasSensor2_list"
 
-(*
-function Chemical_analysis :: "2 Chemical_GasSensor blist[2] \<Rightarrow> Chemical_Status" where
-"Chemical_analysis (bmake TYPE(2) []) =  Chemical_Status_noGas" |
-"Chemical_analysis (bmake TYPE(2) (p#ps)) = 
-  (if Chemical_Chem_is_zero (c p) \<and> (Chemical_analysis (bmake TYPE(2) ps) = Chemical_Status_noGas) 
-   then Chemical_Status_noGas else Chemical_Status_gasD)"
-     apply (auto)
-*)
-
+text \<open>The function @{text analysis} is not specified in the model, but an implemented is defined in 
+the CSP semantics. The definition of @{term Chemical_analysis} is based on the implementation. Since 
+it is defined as a general recursive function, we need to prove its termination. \<close>
 function Chemical_analysis :: "2 Chemical_GasSensor blist[2] \<Rightarrow> Chemical_Status" where
 "Chemical_analysis (gs) = 
   (case list_of_blist gs of
@@ -127,7 +150,10 @@ qed
 value "Chemical_analysis (bmake TYPE(2) [])"
 value "Chemical_analysis (bmake TYPE(2) [\<lparr>c = Chemical_ChemC (0::2), i = Chemical_IntensityC (0::2)\<rparr>])"
 
-text \<open> The intensity function \<close>
+text \<open> The @{text intensity} function in the model is defined using precondition and postconditions. 
+The precondition is evaluated by @{text pre_Chemical_intensity} and its postconditions are 
+established by the function @{term Chemical_intensity} defined below.
+\<close>
 definition pre_Chemical_intensity :: "2 Chemical_GasSensor blist[2] \<Rightarrow> bool" where
 "pre_Chemical_intensity gs = (blength gs > 0)"
 
@@ -152,7 +178,8 @@ value "Chemical_intensity (bmake TYPE(2)
   [\<lparr>c = Chemical_ChemC (0::2), i = Chemical_IntensityC (1::2)\<rparr>,
    \<lparr>c = Chemical_ChemC (1::2), i = Chemical_IntensityC (0::2)\<rparr>])"
 
-text \<open> The location function \<close>
+text \<open> The definition of the @{text location} function in the model is similar to that of the 
+@{text intensity} function.\<close>
 definition pre_Chemical_location :: "2 Chemical_GasSensor blist[2] \<Rightarrow> bool" where
 "pre_Chemical_location gs = (blength gs > 0)"
 
@@ -180,7 +207,7 @@ value "Chemical_location (bmake TYPE(2)
   [\<lparr>c = Chemical_ChemC (0::2), i = Chemical_IntensityC (0::2)\<rparr>,
    \<lparr>c = Chemical_ChemC (1::2), i = Chemical_IntensityC (1::2)\<rparr>])"
 
-subsection \<open> Location package \<close>
+subsection \<open> Location package \label{ssec:chem_location}\<close>
 datatype Location_Loc = 
   Location_Loc_left | Location_Loc_right | Location_Loc_front
 
